src/class_instances.v
@@ -74,9 +74,9 @@ Global Hint Extern 0 (AsRecV (RecV _ _ _) _ _ _) =>
 
 Section pure_exec.
   Local Ltac solve_exec_safe := intros; subst; do 3 eexists; econstructor; eauto.
-  Local Ltac solve_exec_puredet := simpl; intros; by inv_head_step.
+  Local Ltac solve_exec_puredet := simpl; intros; by inv_base_step.
   Local Ltac solve_pure_exec :=
-    subst; intros ?; apply nsteps_once, pure_head_step_pure_step;
+    subst; intros ?; apply nsteps_once, pure_base_step_pure_step;
       constructor; [solve_exec_safe | solve_exec_puredet].
 
   Global Instance pure_recc f x (erec : expr) :
