src/tactics.v
@@ -5,7 +5,7 @@ From iris Require Import options.
 (*|
 This file implements some low-level tactics used to implement simp_lang.
 `reshape_expr` is used to implement the proofmode support (especially tactics
-like `wp_bind` and `wp_pure`) while `inv_head_step` is convenient automation for
+like `wp_bind` and `wp_pure`) while `inv_base_step` is convenient automation for
 proving typeclass instances that describe simp_lang's reduction rules.
 |*)
 
@@ -31,24 +31,24 @@ Ltac reshape_expr e tac :=
   with add_item Ki K e := go (Ki :: K) e
   in go (@nil ectx_item) e.
 
-(** The tactic [inv_head_step] performs inversion on hypotheses of the shape
-[head_step]. The tactic will discharge head-reductions starting from values, and
+(** The tactic [inv_base_step] performs inversion on hypotheses of the shape
+[base_step]. The tactic will discharge head-reductions starting from values, and
 simplifies hypothesis related to conversions from and to values, and finite map
 operations. This tactic is slightly ad-hoc and tuned for proving our lifting
 lemmas. *)
-Ltac inv_head_step :=
+Ltac inv_base_step :=
   repeat match goal with
   | _ => progress simplify_map_eq/= (* simplify memory stuff *)
   | H : to_val _ = Some _ |- _ => apply of_to_val in H
-  | H : head_step ?e _ _ _ _ _ |- _ =>
+  | H : base_step ?e _ _ _ _ _ |- _ =>
      try (is_var e; fail 1); (* inversion yields many goals if [e] is a variable
      and should thus better be avoided. *)
      inversion H; subst; clear H
   end.
 
-Create HintDb head_step.
-Global Hint Extern 0 (head_reducible _ _) => eexists _, _, _, _; simpl : head_step.
+Create HintDb base_step.
+Global Hint Extern 0 (base_reducible _ _) => eexists _, _, _, _; simpl : base_step.
 
 (* [simpl apply] is too stupid, so we need extern hints here. *)
-Global Hint Extern 1 (head_step _ _ _ _ _ _) => econstructor : head_step.
-Global Hint Extern 0 (head_step (HeapOp AllocOp _ _) _ _ _ _ _) => apply alloc_fresh : head_step.
+Global Hint Extern 1 (base_step _ _ _ _ _ _) => econstructor : base_step.
+Global Hint Extern 0 (base_step (HeapOp AllocOp _ _) _ _ _ _ _) => apply alloc_fresh : base_step.
